\documentclass{article}
\usepackage{amsmath}
\begin{document}

\[
A = \begin{bmatrix}
    1 & 2 \\
    3 & 4
\end{bmatrix},
\qquad
B = \begin{bmatrix}
    5 & 6 \\
    7 & 8
\end{bmatrix}
\]

\[
AB = \begin{bmatrix}
    1 & 2 \\
    3 & 4
\end{bmatrix}
\begin{bmatrix}
    5 & 6 \\
    7 & 8
\end{bmatrix}
= \begin{bmatrix}
    (1)(5)+(2)(7) & (1)(6)+(2)(8) \\
    (3)(5)+(4)(7) & (3)(6)+(4)(8)
\end{bmatrix}
= \begin{bmatrix}
    19 & 22 \\
    43 & 50
\end{bmatrix}
\]

\end{document}