\documentclass{article}
\usepackage{musixtex}

\begin{document}
$$\int \frac{2e^{-t^2}}{\sqrt{\pi}} dt = -\frac{2}{\sqrt{\pi}}\int e^{-t^2}d(-t^2)$$

Let $u = -t^2$, then $du = -2t, dt$ and we have:

$$-\frac{2}{\sqrt{\pi}}\int e^{-t^2}d(-t^2) = -\frac{2}{\sqrt{\pi}}\int e^u du = -\frac{2}{\sqrt{\pi}} e^u + C = -\frac{2}{\sqrt{\pi}} e^{-t^2} + C$$

where $C$ is an arbitrary constant of integration.

Now we can evaluate the original limit:

$$\lim_{x\to\infty} \int_{0}^{x} \frac{2e^{-t^2}}{\sqrt{\pi}} dt = \lim_{x\to\infty} \left[-\frac{2}{\sqrt{\pi}} e^{-t^2} \right]{0}^{x} = \lim{x\to\infty} \left[-\frac{2}{\sqrt{\pi}} e^{-x^2} + \frac{2}{\sqrt{\pi}} \right]$$

Since $e^{-x^2}$ approaches zero faster than $x$ approaches infinity, we have:

$$\lim_{x\to\infty} \left[-\frac{2}{\sqrt{\pi}} e^{-x^2} + \frac{2}{\sqrt{\pi}} \right] = \frac{2}{\sqrt{\pi}}$$

Therefore, the limit of the given integral as $x$ approaches infinity is $\frac{2}{\sqrt{\pi}}$.

\end{document}