\documentclass{article}
\usepackage[utf8]{inputenc}
\title{Solution}
\begin{document}
$\int_{-2}^{2}\left( x^{3}cos\frac{x}{2}+\frac{1}{2} \right)\sqrt{4-x^{2}}dx$\\\\\
First, let's make the substitution $x = 2\sin{\theta}$\\\ 
so $dx =2\cos{\theta}d\theta$ and $\sqrt{4-x^2} = 2\cos{\theta}$.\\\\\
Now, we have:\\\\
$\Longrightarrow$ 
$\int_{-2}^{2}\left( x^{3}cos\frac{x}{2}+\frac{1}{2} \right)\sqrt{4-x^{2}}dx$  \\\\\ 
$= \int_{-\frac{\pi}{2}}^{\frac{\pi}{2}}\left( (2\sin{\theta})^{3}\cos\frac{2\sin{\theta}}{2}+\frac{1}{2} \right)(2\cos{\theta})d\theta$ \\\\\ 
$=\int_{-\frac{\pi}{2}}^{\frac{\pi}{2}}\left( 8\sin^{3}{\theta}\cos{\theta}\cos\frac{2\sin{\theta}}{2}+\cos{\theta} \right)d\theta$\\\\\ 
$=\int_{-\frac{\pi}{2}}^{\frac{\pi}{2}}\left( 8\sin^{3}{\theta}\cos{\theta}\cos\sin{\theta}+\cos{\theta} \right)d\theta$\\\\
Now, we can use integration by parts:\\
Let $u = \sin{\theta}$
$dv = 8\sin^{2}{\theta}\cos{\theta}\cos\sin{\theta} + \cos{\theta}d\theta$\\\\\ 
then $du = \cos{\theta}d\theta$\\\\\ 
$v = -\frac{8}{2}\sin^{3}{\theta}\sin\sin{\theta} - \sin{\theta}$\\\\\ 
So, we have:
$\int_{-\frac{\pi}{2}}^{\frac{\pi}{2}}\left( 8\sin^{3}{\theta}\cos{\theta}\cos\sin{\theta}+\cos{\theta} \right)d\theta = [-\frac{8}{2}\sin^{3}{\theta}\sin\sin{\theta} - \sin{\theta}]_{-\frac{\pi}{2}}^{\frac{\pi}{2}}$
$=\frac{8}{2}(0-0) - (-1-1) = 0$\\\
So the definite integral is 0.\\\\

$\frac{\int_{}^{} \left(\sqrt{[5-\sqrt[3]{3}]^{2}_{-2}}\times  \Pi \right)dx}
{\left( \lim_{x \to \infty}\frac{\pi(3) \space \times\space 4}{\frac{\pi}{3}} \right)(4\sqrt{-1})^{5}}\space{\times }\sum_{k=1}^{n=k^{2}} (5)^{4n}\times (n-1)=?$
\end{document}