\documentclass[10pt]{article}
\usepackage[utf8]{inputenc}
\usepackage[T1]{fontenc}
\usepackage{amsmath}
\usepackage{amsfonts}
\usepackage{amssymb}
\usepackage[version=4]{mhchem}
\usepackage{stmaryrd}

\begin{document}
$$
\int \frac{2 e^{2 x}-e^x}{\sqrt{3 e^{2 x}-6 e^x-1}} d x$$

$\int \frac{2 e^{2 x}-e^x}{\sqrt{3 e^{2 x}-6 e^x-1}} d x=\int \frac{\left(2 e^x-1\right) e^x}{\sqrt{3\left(e^{2 x}-2 e^x-\frac{1}{3}\right)}} d x=\int \frac{\left(2 e^x-1\right) e^x}{\sqrt{3} \sqrt{e^{2 x}-2 e^x-\frac{1}{3}}} d x$
$=\frac{1}{\sqrt{3}} \int \frac{\left(2 e^x-1\right) e^x}{\sqrt{e^{2 x}-2 e^x-\frac{1}{3}}} d x$\\
\ u=e\^{}x, d u=$\frac{1}{\sqrt{3}} \int \frac{1}{\sqrt{v^2-\frac{4}{3}}} d v$, let $v=\frac{2}{\sqrt{3}} \sec \theta, d v=\frac{2}{\sqrt{3}} \sec \theta \tan \theta d \theta$
$\frac{1}{\sqrt{3}} \int \frac{\frac{2}{\sqrt{3}} \sec \theta \tan \theta}{\sqrt{\frac{4}{3} \sec ^2 \theta-\frac{4}{3}}} d \theta=\frac{2}{3} \int \frac{\sec \theta \tan \theta}{\sqrt{\frac{4}{3}\left(\sec ^2 \theta-1\right)}}=\frac{2}{3} \int \frac{(\sec \theta \tan \theta)}{\frac{2}{\sqrt{3}} \sqrt{\tan ^2 \theta}} d \theta=$
$e^x d x, \frac{1}{\sqrt{3}} \int \frac{2 u-1}{\sqrt{u^2-2 u-\frac{1}{3}}} d u=\frac{1}{\sqrt{3}}$

$$
\begin{aligned}
& \frac{1}{\sqrt{3}} \int \frac{2 v}{\sqrt{v^2-\frac{4}{3}}} d v+\frac{1}{\sqrt{3}} \int \frac{1}{\sqrt{v^2-\frac{4}{3}}}, w=v^2-\frac{4}{3}, d w=2 v d v \\
& \frac{1}{\sqrt{3}} \int \frac{1}{\sqrt{w}} d w=\frac{1}{\sqrt{3}}(2 \sqrt{w})=\frac{2}{\sqrt{3}} \sqrt{v^2-\frac{4}{3}}= \\
& \frac{2 \sqrt{3}}{3} \sqrt{(u-1)^2-\frac{4}{3}}=\frac{2 \sqrt{3}}{3} \sqrt{u^2-2 u-\frac{1}{3}} \\
& =\frac{2}{3} \sqrt{3 u^2-6 u-1}=\frac{2}{3} \sqrt{3 e^{2 x}-6 e^x-1}
\end{aligned}
$$

\[
\begin{aligned}
& \frac{1}{\sqrt{3}} \int \frac{2 v}{\sqrt{v^2-\frac{4}{3}}} d v+\frac{1}{\sqrt{3}} \int \frac{1}{\sqrt{v^2-\frac{4}{3}}}, w=v^2-\frac{4}{3}, d w=2 v d v \\
& \frac{1}{\sqrt{3}} \int \frac{1}{\sqrt{w}} d w=\frac{1}{\sqrt{3}}(2 \sqrt{w})=\frac{2}{\sqrt{3}} \sqrt{v^2-\frac{4}{3}}= \\
& \frac{2 \sqrt{3}}{3} \sqrt{(u-1)^2-\frac{4}{3}}=\frac{2 \sqrt{3}}{3} \sqrt{u^2-2 u-\frac{1}{3}} \\
& =\frac{2}{3} \sqrt{3 u^2-6 u-1}=\frac{2}{3} \sqrt{3 e^{2 x}-6 e^x-1}
\end{aligned}
\]
\[
\begin{aligned}
& \frac{1}{\sqrt{3}} \ln \left(\frac{e^x \sqrt{3}}{2}-\frac{\sqrt{3}}{2}+\frac{1}{2} \sqrt{3 e^{2 x}-6 e^x-1}\right)= \\
& \frac{1}{\sqrt{3}} \ln \left(\frac{\sqrt{3}}{2}\left(e^x-1+\frac{1}{\sqrt{3}} \sqrt{3 e^{2 x}-6 e^x-1}\right)\right)= \\
& \frac{1}{\sqrt{3}} \ln \left(\frac{\sqrt{3}}{2}\right)+\frac{1}{\sqrt{3}} \ln \left(e^x-1+\sqrt{\frac{3 e^{2 x}-6 e^x-1}{3}}\right) \\
& \frac{2}{3} \sqrt{3 e^{2 x}-6 e^x-1}+\frac{1}{\sqrt{3}} \ln \left(e^x-1+\sqrt{\frac{3 e^{2 x}-6 e^x-1}{3}}\right)+C
\end{aligned}
\]

\end{document}