\documentclass{article}
\usepackage{xfrac,bigints}
\begin{document}
1st Integral
$\int_{0}^{\infty}\left( \frac{x}{sin h(x)}\right)^{2}dx=$
$4\int_{0}^{\infty}\left( \frac{x^{2}}{(e^{x}-e^{-x})^{2}} \right)$
$=4\int_{0}^{\infty}\left( \frac{x^{2}e^{-2x}}{(1-e^{-2x})^{2}} \right)dx$\\\\
$=4\int_{0}^{\infty}\sum_{n=1}^{\infty }x^{2}ne^{-2nx}dx=4\sum_{n=1}^{\infty }n\int_{0}^{\infty}x^2e^{-2nx}dx\\\\
=4\sum_{n=1}^{\infty }n\int_{0}^{\infty}x^2e^{-2nx}dx=4\sum_{n=1}^{\infty }n\int_{0}^{\infty}(\frac{x}{2n})^2e^{-x}\frac{dx}{2n}\\\\
=\frac{1}{2}\sum_{n=1}^{\infty }\frac{1}{n^2}\int_{0}^{\infty}x^2e^{-x}dx=\sum_{n=1}^{\infty}n^{-2}
=\zeta(2)=\frac{\pi^2}{6}$\\\\

2nd Integral
$\int_{0}^{\infty}\left( \frac{x}{sin h(x)}\right)^{2}dx=$
$4\int_{0}^{\infty}\left( \frac{x^{2}}{(e^{x}-e^{-x})^{2}} \right)$
$=4\int_{0}^{\infty}\left( \frac{x^{2}e^{-2x}}{(1-e^{-2x})^{2}} \right)dx$\\\\
$=4\int_{0}^{\infty}\sum_{n=1}^{\infty }x^{2}ne^{-2nx}dx\\\\
=4\sum_{n=1}^{\infty }n\int_{0}^{\infty}x^2e^{-2nx}dx$\\\\
$=4\sum_{n=1}^{\infty }n\int_{0}^{\infty}x^2e^{-2nx}dx\\\\$
$=4\sum_{n=1}^{\infty }n\int_{0}^{\infty}(\frac{x}{2n})^2e^{-x}\frac{dx}{2n}$\\\\$ =\frac{1}{2}\sum_{n=1}^{\infty }\frac{1}{n^2}\int_{0}^{\infty}x^2e^{-x}dx=\sum_{n=1}^{\infty}n^{-2}$\\\\
$=\zeta(2)=\frac{\pi^2}{6}$\\\\
  
\end{document}