\documentclass{article}
\usepackage{amsmath,amssymb}
\usepackage{graphicx}
\usepackage{bigints}
\begin{document}
$
I=\int_{0}^{\infty }\frac{dx}{\sqrt{x}(x^2+(1+2)x+1)(1-x+x^2-x^3...+(-1)^{n}x^{n})}dx\\\\\
I=\int_{0}^{\infty }\frac{(1+x)}{\sqrt{x}(x^2(1+2\sqrt{2})x+4)(x^{n+1}+1)}dx;x \to \frac{1}{x}\\\\
\Rightarrow I=\int_{0}^{\infty}\frac{(1+x)x^{n+1}}{\sqrt{x}(x^2(1+2(1+2\sqrt{2})x+1)(x^{n+1}+1)}dx\\\\
I+I=2I=\int_{0}^{\infty}\frac{(1+x)(1+x^{n+1})(1+x^{n+1}+1)}{\sqrt{x}(x^2+(1+2\sqrt{2})x+1)(x^{n+1}+1)}dx\\\\
\Rightarrow I=\frac{1}{2}\int_{0}^{\infty }\frac{1+x}{\sqrt{x}(x^2+(1+2\sqrt{2})x+1}dx\\\\
\text{let x} = t^{2}\Rightarrow I=\int_{0}^{\infty }\frac{1+t^{2}}{t^{4}+(1+2\sqrt{2})t^2+1}dt\\\\
=\int_{0}^{\infty }\frac{1+t^2}{t^4+dt^2+1}dt;\text{where d=1+2}\sqrt{2}\\\\
\text{let t}= tan\theta\Rightarrow I=\int_{0}^{\frac{\pi}{2}}\frac{(1+tan^{2}\theta)^2}{tan^4\theta+dtan^2\theta+1}d\theta\\\\
=\int_{0}^{\frac{\pi}{2}}\frac{d\theta}{sin^4\theta+cos^4\theta+dsin^2\theta cos^\theta};\text{then:}\\\\
I=\int_{0}^{\frac{\pi}{2}}\frac{d\theta}{1-2sin^2\theta cos^2\theta+sin^2\theta cos^2\theta}\\\\
=\int_{0}^{\frac{\pi}{2}}\frac{d\theta}{1+(d-2)sin^2\theta cos^2\theta}
=\int_{0}^{\frac{\pi}{2}} \frac{d\theta}{1+\frac{d-2}{4}sin^2(2\theta)}; then:\\\\
I=4\int_{0}^{\pi}\frac{d4}{(6+d)+(2-d)cos\varphi}:\\\\
\text{let I(a:b) =}\int_{0}^{\pi}\frac{d\varphi}{a+bcos\varphi}:t=tan(\frac{\varphi}{2}):\\\\ 
I(a\cdot b)=\int_{0}^{\infty}\frac{2dt}{(a+b)+(a\cdot b)t^2}\\\\
I(a:b)=\frac{2}{a-b}\int_{0}^{\infty}\frac{dt}{\frac{a+b}{a-b}+t^2}\\\\
=\frac{\pi}{\sqrt{a^2-b^2}}; I=4(6+d;2-d)\\\\
= \frac{4\pi}{\sqrt{(6+d)^2-(2-d)^2}}=\frac{\pi}{\sqrt{d+2}}\\\\
I=\frac{\pi}{\sqrt{1+2\sqrt{2}+2}}=\frac{\pi}{\sqrt{3+2\sqrt{2}}}=\frac{\pi}{\sqrt{(1+\sqrt{2})^2}}\\\\ 
= \frac{\pi}{1+\sqrt{2}}\\\\
$
\end{document}