\documentclass{article}
\usepackage{amsmath,amssymb}
\usepackage{graphicx}
\usepackage{bigints}
\begin{document}
$
I = \int_{0}^{\frac{\pi}{2}}ln(cos(x))dx=\\\\
\\
I = \int_{0}^{\frac{\pi}{2}}ln(cos(x))dx=
           \int_{0}^{\frac{\pi}{2}}ln(cos(\frac{\pi}{2}-2))dx
           =\int_{0}^{\frac{\pi}{2}}ln(sin(x))dx\\\\
2 I = \int_{0}^{\frac{\pi}{2}}ln(cos(x))dx+ln(sin(x))dx\\\\
= \int_{0}^{\frac{\pi}{2}}ln(sin(x)cos(x))dx= \int_{0}^{\frac{\pi}{2}}ln(\frac{1}{2}sin(2x))dx\\\\
= \int_{0}^{\frac{\pi}{2}} ln\left( \frac{1}{2} \right)dx + \int_{0}^{\frac{\pi}{2}}(sin(2x))dx\\\\
= \frac{\pi}{2}ln\left( \frac{1}{2} \right)+\frac{1}{2}\int_{0}^{\frac{\pi}{2}} sin(x)dx\\\\
= \frac{\pi}{2}ln\left( \frac{1}{2} \right)+\frac{1}{2}\int_{0}^{\frac{\pi}{2}} sin(x)dx+\frac{1}{2}\int_{\frac{\pi}{2}}^{n}sin(x)dx\\\\
=\frac{\pi}{2}ln\left(\frac{1}{2}\right)+\frac{1}{2}I+\frac{1}{2}\int_{0}^{\frac{\pi}{2}}cos(x)dx\\\\
2I=\frac{\pi}{2}ln\left( \frac{1}{2}\right)+I\\\\
I=\frac{\pi}{2}ln\left( \frac{1}{2}\right)= \int_{0}^{\frac{\pi}{2}}ln(cos(x))dx
$\\\\

\end{document}