\documentclass{article}
\usepackage{amsmath}
\usepackage{titlesec}
\usepackage{xcolor}
\usepackage[dvipsnames]{xcolor}
\title{\color{blue}Mathematical Analysis of a Triple Integral using Gamma Function and Binomial Series}
\author{Kensukeken}
\date{April 1, 2023}

\begin{document}

\maketitle
\[
\int_{\theta_1}^{\theta_2}\int_{y_1}^{y_2}\int_{0}^{\infty}\frac{t^{a-1}\sum_{p=0}^{n}\frac{(n)p}{p!}e^{(n-p-b)^{t}}r^{p}\cos[(m-p)\theta]}{(e^{2t}+2re^{t}\cos \theta +r^{2})^{r}}\, dt\, dr\, d\theta
\]

\text{Some notation, formulas and theorems used in this paper are introduced below.}
\subsection {Notations}
\subsection{Gamma Function}
\text{Suppose that a is a postive real number, then}
$\Gamma(a)= \int_{0}^{\infty}t^{a-1}e^{-t}$
\subsection{} $(s)_k=s(s-1)\cdot \cdot \cdot (s-k+1),$ \text{where s is a real number.}
\section{Formulas}
\subsection{Euler's Formula}
$e^{ix}= cos(x)+i sin(x), \text{where x is any real number.}$
\subsubsection{Demoivre's Formula}
$(cos(x) +sin(x)^2=cos(nx)+isin(nx),\text{ where n is any interger, and x is any real number.}$
\section{Theorems}
\text{Two important theorems used in this study are introduced}
\subsection{Bionomial Series}
$(1+z)^s=\sum_{k=0}^{\infty}\frac{(s)_{k}}{k!}z^{k}$ \text{, where z is a complex number, [z]$<$1, and s is a real number.}
\subsection{Integration Terms by Term Theorem}
\text{Suppose that $\left\{ g_{n} \right\}\mathrm{}_{n=0}^{\infty}$ is a sequence of Lebesgue interable function defined on I.} 
\text{If $\sum_{n=0}^{\infty}\int_{I}^{}|g_{n}|$ \text{ is convergent, then}} \\
\text{$\int_{I}^{}\sum_{n=1}^{\infty }g_{n}=\sum_{n=0}^{\infty }\int_{I}^{}g_{n}$}
\text{Before deriving the major results of this study, wee need a lemma.}


\section{Lemma}
\subsection{Lemma}

\text{Suppose that z is a complex number, [z]$<$1, a,b are real numbers, a>0, b$\ge$0, and m.n are postive integers. Then the improper integeral:}\\\\

$\int_{0}^{\infty }\frac{t^{a-1}e^{-bt}z^m}{(e^{t}+z)^n}dt=\Gamma(a)\sum_{k=0}^{\infty}\frac{(-n)_k}{k!(k+n+b)^a}z^{k+m}$\\\\
\\
$\frac{t^{a+1}e^{-bt}z^m}{(e^{t}+z)^n}=t^{a-1}e^{-bt}e^{-nt}z^m \cdot \frac{1}{\left( 1+\frac{z}{e^t} \right)^n}$
$=t^{a+1}e^{-(n+b)t}z^m \cdot \sum_{k=0}^{\infty}\frac{(-n)_k}{k!}e^{-kt}z^k
$

\text{(by binomial series)}

$=\sum_{k=0}^{\infty }\frac{(-n)k}{k!}t^{a-1}e^{-(k+n+b)t}z^{k+m}$
\\\\
\begin{align}
\int_{0}^{\infty }\frac{t^{a-1}e^{-bt}z^m}{(e^t+z)^n}dt\\
= \int_{0}^{\infty }\sum_{k=0}^{\infty }\frac{(-n)_k}{k!}t^{a-1}e^{-(k+n+b)t}z^{k+m}dt\\
=\sum_{k=0}^{\infty }\frac{(-n)_k}{k!}\left( \int_{0}^{\infty } t^{a-1}e^{(-k+n+n)t}dt\right)z^{k+m}\\
\Gamma(a)\cdot \sum_{k=0}^{\infty }\frac{(-n)_k}{k!(k+n+b)a}z^{k+m}
\end{align}
\text{Firstly, we determine the infinete series form of the triple integral(1).}
\subsection{Theorem}
\text{Assume that $r_1$, $r_2$, $theta_1$, $\theta_2$ are real numbers, [$r_1$]$<$1,  [$r_2$]$\lt$1, a,b are real numbers, a $>$ 0, b $\ge$0,} 
\text{m.n are positive intefers. Then the triple integral: }\\\\
\[\int_{\theta_1}^{\theta_2}\int_{y_1}^{y_2}\int_{0}^{\infty}\frac{t^{a-1}\sum_{p=0}^{n}\frac{(n)p}{p!}e^{(n-p-b)^{t}}r^{p}cos[(m-p)\theta]}{(e^{2t}+2re^{t}cos \theta +r^{2})^{r}}dtdrd\theta
\]

\\\
See page 3 for the solution and explanation
\newpage
\thetitle{ Contiuned}
\[\int_{\theta_1}^{\theta_2}\int_{y_1}^{y_2}\int_{0}^{\infty}\frac{t^{a-1}\sum_{p=0}^{n}\frac{(n)p}{p!}e^{(n-p-b)^{t}}r^{p}cos[(m-p)\theta]}{(e^{2t}+2re^{t}cos \theta +r^{2})^{r}}dtdrd\theta 
\]

\[
(-n)_k(r2^{k+1}-r1^{k+1})
\]
\[
=\Gamma(a) \cdot \sum_{k=0}^{\infty}\frac{[sin(k+m)\theta2-sin(k+m)\theta 1]}{k!(k+1)(k+m)(k+n+b)^{a}}
\]
\text{Proof Let z= re^{i$\theta$}}
\[
\int_{0}^{\infty }\frac{t^{a-1}e^{-bt}(re^{i\theta})^m}{(e^t +re^{i\theta})^n}dt\\
\]

\[
=\Gamma(a) \cdot \sum_{k=0}^{\infty }\frac{(-n)_k}{k!(k+n+b)^a}(re^{i\theta})^{k+m}
\]
\text{By Euler's formula and DeMoivre's formula, we obtain:}\\

\[
\int_{0}^{\infty }\frac{t^{a-1}e^{-bt}e^{im(\theta)}(e^ +re^{-i\theta})^n}{(e^2t+2re^t cos\theta +r^2)^a}dt\\
=\Gamma(a)\cdot \sum_{k=0}^{\infty}\frac{(-n)_k}{k!(k+n+b)^a}r^ke^i(k+m)\theta\\  
\]
\text{Therefore,}
\[
\int_{0}^{\infty }\frac{t^{a-1}\sum_{p=0}^{n}e^{(n-p-b)^t}r^p e^{i(m-p)\theta}}{(e^2t+2re^tcos\theta +r^2)^n}dt\\
\]


\[
=\Gamma(a)\cdot \sum_{k=0}^{\infty}\frac{(-n)_k}{k!(k+n+b)^a}r^k e^{i(k+m)\theta}
\]
\end{document}